thy/IP_Addresses/WordInterval_Lists.thy
@@ -4,26 +4,26 @@ imports WordInterval
 begin
 
 
-  fun l2br_negation_type_union :: "('a::len word \<times> 'a::len word) negation_type list \<Rightarrow> 'a::len wordinterval" where
-    "l2br_negation_type_union [] = Empty_WordInterval" |
-    "l2br_negation_type_union ((Pos (s,e))#ls) = wordinterval_union (WordInterval s e) (l2br_negation_type_union ls)" |
-    "l2br_negation_type_union ((Neg (s,e))#ls) = wordinterval_union (wordinterval_invert (WordInterval s e)) (l2br_negation_type_union ls)"
+  fun l2wi_negation_type_union :: "('a::len word \<times> 'a::len word) negation_type list \<Rightarrow> 'a::len wordinterval" where
+    "l2wi_negation_type_union [] = Empty_WordInterval" |
+    "l2wi_negation_type_union ((Pos (s,e))#ls) = wordinterval_union (WordInterval s e) (l2wi_negation_type_union ls)" |
+    "l2wi_negation_type_union ((Neg (s,e))#ls) = wordinterval_union (wordinterval_invert (WordInterval s e)) (l2wi_negation_type_union ls)"
 
 
-  lemma l2br_negation_type_union: "wordinterval_to_set (l2br_negation_type_union l) = 
+  lemma l2wi_negation_type_union: "wordinterval_to_set (l2wi_negation_type_union l) = 
                         (\<Union> (i,j) \<in> set (getPos l). {i .. j}) \<union> (\<Union> (i,j) \<in> set (getNeg l). - {i .. j})"
-  apply(simp add: l2br)
-  apply(induction l rule: l2br_negation_type_union.induct)
+  apply(simp add: l2wi)
+  apply(induction l rule: l2wi_negation_type_union.induct)
     apply(simp_all)
    apply fast+
   done
 
 
 
- definition l2br_intersect :: "('a::len word \<times> 'a::len word) list \<Rightarrow> 'a::len wordinterval" where
-    "l2br_intersect = foldl (\<lambda> acc (s,e). wordinterval_intersection (WordInterval s e) acc) wordinterval_UNIV"
+ definition l2wi_intersect :: "('a::len word \<times> 'a::len word) list \<Rightarrow> 'a::len wordinterval" where
+    "l2wi_intersect = foldl (\<lambda> acc (s,e). wordinterval_intersection (WordInterval s e) acc) wordinterval_UNIV"
 
-  lemma l2br_intersect: "wordinterval_to_set (l2br_intersect l) = (\<Inter> (i,j) \<in> set l. {i .. j})"
+  lemma l2wi_intersect: "wordinterval_to_set (l2wi_intersect l) = (\<Inter> (i,j) \<in> set l. {i .. j})"
     proof -
     { fix U --\<open>@{const wordinterval_UNIV} generalized\<close>
       have "wordinterval_to_set (foldl (\<lambda>acc (s, e). wordinterval_intersection (WordInterval s e) acc) U l) = (wordinterval_to_set U) \<inter> (\<Inter>(i, j)\<in>set l. {i..j})"
@@ -31,26 +31,26 @@ begin
            apply(simp)
           by force
     } thus ?thesis
-      unfolding l2br_intersect_def by simp
+      unfolding l2wi_intersect_def by simp
     qed
 
 
-  fun l2br_negation_type_intersect :: "('a::len word \<times> 'a::len word) negation_type list \<Rightarrow> 'a::len wordinterval" where
-    "l2br_negation_type_intersect [] = wordinterval_UNIV" |
-    "l2br_negation_type_intersect ((Pos (s,e))#ls) = wordinterval_intersection (WordInterval s e) (l2br_negation_type_intersect ls)" |
-    "l2br_negation_type_intersect ((Neg (s,e))#ls) = wordinterval_intersection (wordinterval_invert (WordInterval s e)) (l2br_negation_type_intersect ls)"
+  fun l2wi_negation_type_intersect :: "('a::len word \<times> 'a::len word) negation_type list \<Rightarrow> 'a::len wordinterval" where
+    "l2wi_negation_type_intersect [] = wordinterval_UNIV" |
+    "l2wi_negation_type_intersect ((Pos (s,e))#ls) = wordinterval_intersection (WordInterval s e) (l2wi_negation_type_intersect ls)" |
+    "l2wi_negation_type_intersect ((Neg (s,e))#ls) = wordinterval_intersection (wordinterval_invert (WordInterval s e)) (l2wi_negation_type_intersect ls)"
 
-  lemma l2br_negation_type_intersect_alt: "wordinterval_to_set (l2br_negation_type_intersect l) = 
-                  wordinterval_to_set (wordinterval_setminus (l2br_intersect (getPos l)) (l2br (getNeg l)))"
-    apply(simp add: l2br_intersect l2br)
-    apply(induction l rule :l2br_negation_type_intersect.induct)
+  lemma l2wi_negation_type_intersect_alt: "wordinterval_to_set (l2wi_negation_type_intersect l) = 
+                  wordinterval_to_set (wordinterval_setminus (l2wi_intersect (getPos l)) (l2wi (getNeg l)))"
+    apply(simp add: l2wi_intersect l2wi)
+    apply(induction l rule :l2wi_negation_type_intersect.induct)
        apply(simp_all)
       apply(fast)+
     done
 
-  lemma l2br_negation_type_intersect: "wordinterval_to_set (l2br_negation_type_intersect l) = 
+  lemma l2wi_negation_type_intersect: "wordinterval_to_set (l2wi_negation_type_intersect l) = 
                         (\<Inter> (i,j) \<in> set (getPos l). {i .. j}) - (\<Union> (i,j) \<in> set (getNeg l). {i .. j})"
-    by(simp add: l2br_negation_type_intersect_alt l2br_intersect l2br)
+    by(simp add: l2wi_negation_type_intersect_alt l2wi_intersect l2wi)
 
 
 end
