thy/IP_Addresses/WordInterval_Sorted.thy
@@ -6,10 +6,10 @@ begin
 
 (*TODO: has afp mergesort dependency*)
 definition wordinterval_sort :: "'a::len wordinterval \<Rightarrow> 'a::len wordinterval" where
-  "wordinterval_sort w \<equiv> l2br (mergesort_remdups (br2l w))"
+  "wordinterval_sort w \<equiv> l2wi (mergesort_remdups (wi2l w))"
 
 lemma wordinterval_sort: "wordinterval_to_set (wordinterval_sort w) = wordinterval_to_set w"
-  by (simp add: wordinterval_sort_def br2l l2br mergesort_remdups_correct)
+  by (simp add: wordinterval_sort_def wi2l l2wi mergesort_remdups_correct)
 
 
 end
